test/Main.hs
@@ -13,19 +13,15 @@ Haskell code that was extracted from Coq.
 
 import Tempest
 import Test.Hspec
-import Test.Tasty
-import Test.Tasty.Hspec
 
 main :: IO ()
-main = makeTests >>= defaultMain
-
-makeTests :: IO TestTree
-makeTests = testSpec "Main tests" $
+main = hspec $ do
   describe "Sanity tests" sanityTests
+  describe "Block tests" blockTests
 
 sanityTests :: SpecWith ()
 sanityTests = do
-  it "Single instruction" $ asmTest
+  it "Single instruction" $ asmTest 32
     (label "entry"
         (add v0 v1 v2)
         return_) $
@@ -34,7 +30,7 @@ sanityTests = do
         (add r0 r1 r2)
         return_
 
-  it "Single, repeated instruction" $ asmTest
+  it "Single, repeated instruction" $ asmTest 32
     (label "entry"
         (do add v0 v1 v2
             add v0 v1 v2
@@ -47,7 +43,7 @@ sanityTests = do
             add r0 r1 r2)
         return_
 
-  it "Multiple instructions" $ asmTest
+  it "Multiple instructions" $ asmTest 32
     (label "entry"
         (do add v0 v1 v2
             add v0 v1 v3
@@ -60,7 +56,7 @@ sanityTests = do
             add r0 r1 r2)
         return_
 
-  it "More variables used than registers" $ asmTest
+  it "More variables used than registers" $ asmTest 32
     (label "entry"
         (do add v0 v1 v2
             add v3 v4 v5
@@ -91,7 +87,7 @@ sanityTests = do
             add r22 r23 r10)
         return_
 
-  it "Single long-lived variable" $ asmTest
+  it "Single long-lived variable" $ asmTest 32
     (label "entry"
         (do add v0 v1 v2
             add v0 v4 v5
@@ -106,7 +102,7 @@ sanityTests = do
             add r0 r4 r3)
         return_
 
-  it "Two long-lived variables" $ asmTest
+  it "Two long-lived variables" $ asmTest 32
     (label "entry"
         (do add v0 v1 v2
             add v0 v4 v5
@@ -121,7 +117,7 @@ sanityTests = do
             add r0 r2 r5)
         return_
 
-  it "One variable with a long interval" $ asmTest
+  it "One variable with a long interval" $ asmTest 32
     (label "entry"
         (do add v0   v1  v2
             add v3   v4  v5
@@ -152,7 +148,7 @@ sanityTests = do
             add r0 r22 r11)
         return_
 
-  it "Many variables with long intervals" $ asmTest
+  it "Many variables with long intervals" $ asmTest 32
     (label "entry"
         (do add v0   v1  v2
             add v3   v4  v5
@@ -199,7 +195,7 @@ sanityTests = do
             add r18 r19 r29)
         return_
 
-  it "Spilling one variable" $ asmTest
+  it "Spilling one variable" $ asmTest 32
     (label "entry"
         (do {-  1 -} add v0   v1  v2
             {-  3 -} add v3   v4  v5
@@ -242,7 +238,7 @@ sanityTests = do
             -- registers.  So we pick the first register, counting from 0,
             -- whose next use position is the furthest from this position.
             -- That happens to be r18, which is next used at position 41.
-                     save 18 0
+                     save r18 0
             {- 21 -} add r20 r21 r18
             {- 23 -} add r0 r1 r22
             {- 25 -} add r2 r3 r23
@@ -257,7 +253,111 @@ sanityTests = do
             -- When it comes time to reload v29 (which had been allocated
             -- to r18), we pick the first available register which happens
             -- to be r0 in this case.
-                     restore 0 0
+                     restore 0 r0
             {- 41 -} add r0 r19 r31
             {- 43 -} add r20 r21 r18)
         return_
+
+blockTests :: SpecWith ()
+blockTests = do
+  it "Allocates across blocks" $ asmTest 32
+    (do label "entry"
+            (add v0 v1 v2)
+            (jump "skipped")
+        label "skipped"
+            (do add v2 v3 v4
+                add v2 v4 v5)
+            (jump "next")
+        label "next"
+            (do add v2 v5 v6
+                add v2 v6 v7
+                add v2 v7 v8)
+            return_)
+
+    (do label "entry"
+            (add r0 r1 r3)
+            (jump "skipped")
+        label "skipped"
+            (do add r3 r2 r0
+                add r3 r0 r1)
+            (jump "next")
+        label "next"
+            (do add r3 r1 r0
+                add r3 r0 r1
+                add r3 r1 r0)
+            return_)
+
+  it "Inserts resolving moves" $ asmTest 4
+    (do label "entry"                           -- 1
+            (add v0 v1 v2)                      -- 3
+            (branch Zero v2 "B3" "B2")          -- 5
+        label "B2"                              -- 7
+            (do add v1 v2 v3                    -- 9
+                add v0 v0 v4                    -- 11
+                add v0 v0 v5                    -- 13
+                add v0 v4 v6                    -- 15
+                add v0 v5 v6)                   -- 17
+            (jump "B4")                         -- 19
+        label "B3"                              -- 21
+            (add v1 v2 v3)                      -- 23
+            (jump "B4")                         -- 25
+        label "B4"                              -- 27
+            (add v3 v3 v0)                      -- 29
+            return_)                            -- 31
+
+    (do label "entry"
+            (add r0 r1 r2)
+            (branch Zero r2 "B2" "B3")
+        label "B2"
+            (add r1 r2 r3)
+            (jump "B4")
+        label "B3"
+            (do add r1 r2 r3
+                save r3 0
+                add r0 r0 r1
+                add r0 r0 r2
+                add r0 r1 r3
+                add r0 r2 r3
+                restore 0 r3)
+            (jump "B4")
+        label "B4"
+            (add r3 r3 r0)
+            return_)
+
+  it "Inserts resolving moves another way" $ asmTest 4
+    (do label "entry"                           -- 1
+            (add v0 v1 v2)                      -- 3
+            (branch Zero v2 "B3" "B2")          -- 5
+        label "B2"                              -- 7
+            (add v1 v2 v3)                      -- 9
+            (jump "B4")                         -- 11
+        label "B3"                              -- 13
+            (do add v1 v2 v3                    -- 15
+                add v0 v0 v4                    -- 17
+                add v0 v0 v5                    -- 19
+                add v0 v4 v6                    -- 21
+                add v0 v5 v6)                   -- 23
+            (jump "B4")                         -- 25
+        label "B4"                              -- 27
+            (add v3 v3 v0)                      -- 29
+            return_)                            -- 31
+
+    (do label "entry"
+            (add r0 r1 r2)
+            (branch Zero r2 "B2" "B3")
+        label "B2"
+            (do add r1 r2 r3
+                save r3 0
+                add r0 r0 r1
+                add r0 r0 r2
+                add r0 r1 r3
+                add r0 r2 r3
+                restore 0 r1)
+            (jump "B4")
+        label "B3"
+            (do add r1 r2 r3
+                move r3 r1)
+            (jump "B4")
+        label "B4"
+            (add r1 r1 r0)
+            return_)
