Assign.v
@@ -23,8 +23,10 @@ Variable binfo : BlockInfo blockType1 blockType2 opType1 opType2.
 Variable oinfo : OpInfo maxReg accType opType1 opType2.
 
 Record AssnStateInfo := {
-  assnOpId : OpId;
-  assnAcc  : accType
+  assnOpId     : OpId;
+  assnBlockBeg : OpId;
+  assnBlockEnd : OpId;
+  assnAcc      : accType
 }.
 
 Definition AssnState := State AssnStateInfo.
@@ -32,22 +34,28 @@ Definition AssnState := State AssnStateInfo.
 Definition moveOpM sreg dreg : AssnState (seq opType2) :=
   assn <-- get ;;
   let: (mop, acc') := moveOp oinfo sreg dreg (assnAcc assn) in
-  put {| assnOpId := assnOpId assn
-       ; assnAcc  := acc' |} ;;
+  put {| assnOpId     := assnOpId assn
+       ; assnBlockBeg := assnBlockBeg assn
+       ; assnBlockEnd := assnBlockEnd assn
+       ; assnAcc      := acc' |} ;;
   pure mop.
 
 Definition saveOpM vid reg : AssnState (seq opType2) :=
   assn <-- get ;;
   let: (sop, acc') := saveOp oinfo vid reg (assnAcc assn) in
-  put {| assnOpId := assnOpId assn
-       ; assnAcc  := acc' |} ;;
+  put {| assnOpId     := assnOpId assn
+       ; assnBlockBeg := assnBlockBeg assn
+       ; assnBlockEnd := assnBlockEnd assn
+       ; assnAcc      := acc' |} ;;
   pure sop.
 
 Definition restoreOpM vid reg : AssnState (seq opType2) :=
   assn <-- get ;;
   let: (rop, acc') := restoreOp oinfo vid reg (assnAcc assn) in
-  put {| assnOpId := assnOpId assn
-       ; assnAcc  := acc' |} ;;
+  put {| assnOpId     := assnOpId assn
+       ; assnBlockBeg := assnBlockBeg assn
+       ; assnBlockEnd := assnBlockEnd assn
+       ; assnAcc      := acc' |} ;;
   pure rop.
 
 Definition pairM {A B : Type} (x : AssnState A) (y : AssnState B) :
@@ -56,19 +64,35 @@ Definition pairM {A B : Type} (x : AssnState A) (y : AssnState B) :
   y' <-- y ;;
   pure (x', y').
 
-Definition savesAndRestores (opid : OpId) vid reg int :
+Definition savesAndRestores (opid : OpId) v reg int :
   AssnState (seq opType2 * seq opType2) :=
+  if @varId maxReg v isn't inr vid then pure ([::], [::]) else
+
+  (* Wimmer: "If a split position is moved to a block boundary, the algorithm
+     for resolving the data flow takes care of inserting the move. It is also
+     possible that no move is necessary at all because of the control flow." *)
+  assn <-- get ;;
+  (* We increment by two before checking the beginning in order to skip past
+     the label. *)
+  let knd := varKind v in
+  let atBoundary :=
+      ((knd == Input)  && (assnBlockBeg assn == opid)) ||
+      ((knd == Output) && (opid.+2 == assnBlockEnd assn)) in
+  if atBoundary then pure ([::], [::]) else
+
   let isFirst := firstUsePos int == Some opid in
   let isLast  := nextUseAfter int opid == None in
   let save    := saveOpM reg (Some vid) in
   let restore := restoreOpM (Some vid) reg in
-  match iknd int, isFirst, isLast with
-    | Middle,    true,  true  => pairM restore save
-    | Middle,    false, true  => pairM (pure [::]) save
-    | Middle,    true,  false => pairM restore (pure [::])
-    | LeftMost,  _,     true  => pairM (pure [::]) save
-    | RightMost, true,  _     => pairM restore (pure [::])
-    | _,         _,     _     => pure ([::], [::])
+  match knd, iknd int, isFirst, isLast with
+    | Input,  LeftMost,  _,     true  => pairM (pure [::]) save
+    | Input,  Middle,    true,  true  => pairM restore save
+    | Input,  Middle,    true,  _     => pairM restore (pure [::])
+    | Input,  Middle,    _,     true  => pairM (pure [::]) save
+    | Input,  RightMost, true,  _     => pairM restore (pure [::])
+    | Output, LeftMost,  _,     true  => pairM (pure [::]) save
+    | Output, Middle,    _,     true  => pairM (pure [::]) save
+    | _,      _,         _,     _     => pure ([::], [::])
     end.
 
 Definition collectAllocs opid ints acc v :=
@@ -80,7 +104,7 @@ Definition collectAllocs opid ints acc v :=
                       seq opType2 * seq opType2) with
     | (int, reg) =>
       let: (allocs', restores', saves') := acc' in
-      res <-- savesAndRestores opid vid reg int ;;
+      res <-- savesAndRestores opid v reg int ;;
       let: (rs, ss) := res in
       pure ((vid, reg) :: allocs', rs ++ restores', ss ++ saves')
     end.
@@ -93,51 +117,67 @@ Definition doAllocations ints op : AssnState (seq opType2) :=
   let: (allocs, restores, saves) := res in
   let op' := applyAllocs oinfo op allocs in
   (* With lenses, this would just be: assnOpId += 2 *)
-  modify (fun assn' => {| assnOpId := opid.+2
-                        ; assnAcc  := assnAcc assn' |}) ;;
+  modify (fun assn' =>
+            {| assnOpId     := opid.+2
+             ; assnBlockBeg := assnBlockBeg assn'
+             ; assnBlockEnd := assnBlockEnd assn'
+             ; assnAcc      := assnAcc assn' |}) ;;
   pure $ restores ++ op' ++ saves.
 
 
-Definition generateMoves (moves : seq (option PhysReg * option PhysReg)) :
+Definition generateMoves
+  (moves : seq (option (PhysReg + nat) * option (PhysReg + nat))) :
   AssnState (seq opType2) :=
   forFoldM [::] moves $ fun acc mv =>
     mops <-- match mv with
-      | (Some sreg, Some dreg) => fmap (@Some _) $ moveOpM sreg dreg
-      | (Some sreg, None)      => fmap (@Some _) $ saveOpM sreg None
-      | (None, Some dreg)      => fmap (@Some _) $ restoreOpM None dreg
-      | (None, None)           => pure None
+      | (Some (inl sreg), Some (inl dreg)) =>
+          fmap (@Some _) $ moveOpM sreg dreg
+      | (Some (inl sreg), Some (inr vid)) =>
+          fmap (@Some _) $ saveOpM sreg (Some vid)
+      | (Some (inl sreg), None) => fmap (@Some _) $ saveOpM sreg None
+      | (Some (inr vid), Some (inl dreg)) =>
+          fmap (@Some _) $ restoreOpM (Some vid) dreg
+      | (None, Some (inl dreg)) => fmap (@Some _) $ restoreOpM None dreg
+        (* jww (2015-02-14): There are possibilities, like Some (inr sv), Some
+           (inr dv), which should be provably impossible, since no resolving
+           move for the same variable would ever both to copy from and to the
+           same stack location. *)
+      | (_, _) => pure None
       end ;;
     pure $ if mops is Some ops then ops ++ acc else acc.
 
-Definition resolveMappings bid ops ops' mappings :
+Definition resolveMappings bid opsm mappings :
   AssnState (seq opType2) :=
   (* Check whether any boundary transitions require move resolution at the
      beginning or end of the block given by [bid]. *)
-  if IntMap_lookup bid mappings isn't Some graphs then pure ops' else
+  if IntMap_lookup bid mappings isn't Some graphs then pure opsm else
 
   let: (gbeg, gend) := graphs in
 
   bmoves <-- generateMoves (topsort gbeg) ;;
-  let ops'' := bmoves ++ ops' in
+  let opsm' := bmoves ++ opsm in
 
   emoves <-- generateMoves (topsort gend) ;;
-  pure $ match ops, ops'' with
-    | o :: os, o'' :: os'' =>
-        if opKind oinfo (last o os) is IsBranch
-        then belast o'' os'' ++ emoves ++ [:: last o'' os'']
-        else ops'' ++ emoves
-    | _, _ => ops'' ++ emoves
-  end.
+  let opsm'' := opsm' ++ emoves in
+  pure opsm''.
 
 Definition considerOps (f : opType1 -> AssnState (seq opType2)) mappings :=
   mapM $ fun blk =>
     (* First apply all allocations *)
     let ops := blockOps binfo blk in
-    ops' <-- concatMapM f ops ;;
+    let: (opsb, opsm, opse) := ops in
+    modify (fun assn =>
+              {| assnOpId     := assnOpId assn
+               ; assnBlockBeg := assnOpId assn + (size opsb).*2
+               ; assnBlockEnd := assnOpId assn + (size opsb + size opsm).*2
+               ; assnAcc      := assnAcc assn |}) ;;
+    opsb' <-- concatMapM f opsb ;;
+    opsm' <-- concatMapM f opsm ;;
+    opse' <-- concatMapM f opse ;;
     (* Insert resolving moves based on the mappings *)
     let bid := blockId binfo blk in
-    ops'' <-- resolveMappings bid ops ops' mappings ;;
-    pure $ setBlockOps binfo blk ops''.
+    opsm'' <-- resolveMappings bid opsm' mappings ;;
+    pure $ setBlockOps binfo blk opsb' opsm'' opse'.
 
 Definition assignRegNum `(st : ScanState InUse sd)
   (mappings : IntMap (BlockMoves maxReg)) (blocks : seq blockType1)
@@ -149,8 +189,10 @@ Definition assignRegNum `(st : ScanState InUse sd)
          | x <- handled sd ++ active sd ++ inactive sd])
       mappings
       blocks
-      {| assnOpId := 1
-       ; assnAcc := acc |} in
+      {| assnOpId     := 1
+       ; assnBlockBeg := 1
+       ; assnBlockEnd := 1
+       ; assnAcc      := acc |} in
   (blocks', assnAcc assn).
 
 End Assign.
